src/Manifest_Set.v
@@ -303,14 +303,14 @@ Proof.
     + apply manadd_In_set in H; destruct H; subst; auto with *.       
 Qed.
 
-Fixpoint manifest_set_to_list_InJson {A :Type} `{Serializable A} 
-    (m : manifest_set A) : list InnerJSON :=
+Fixpoint manifest_set_to_list_InJson {A :Type} `{Stringifiable A} 
+    `{EqClass A} (m : manifest_set A) : list InnerJSON :=
   match m with
   | nil => []
   | h :: t => (InJSON_String (to_string h)) :: (manifest_set_to_list_InJson t)
   end.
 
-Fixpoint list_InJson_to_manifest_set {A :Type} `{Serializable A} `{EqClass A}
+Fixpoint list_InJson_to_manifest_set {A :Type} `{Stringifiable A} `{EqClass A}
     (l : list InnerJSON) : ResultT (manifest_set A) string :=
   match l with
   | nil => resultC []
@@ -320,25 +320,33 @@ Fixpoint list_InJson_to_manifest_set {A :Type} `{Serializable A} `{EqClass A}
       match (list_InJson_to_manifest_set t) with
       | resultC t' => 
           match (from_string s) with
-          | resultC h' => resultC (manset_add h' t')
+          (* TODO: This should really use a safer add, but man sets arent guarded inductively so in proofs the fact is lost for resolution *)
+          | resultC h' => resultC (h' :: t')
           | errC e => errC e
           end
       | errC e => errC e
       end
-    | _ => errC "Error: Invalid JSON type in manifest set, only can handle strings."%string
+    | _ => errC "list_InJson_to_manifest_set: Invalid JSON type in manifest set, only can handle strings."%string
     end
   end.
 
-Fixpoint manifest_set_pairs_to_list_InJson {A B : Type} `{Serializable A} 
-    `{Serializable B} (m : manifest_set (A * B)) : list InnerJSON :=
+Lemma canonical_list_injson_to_manset {A : Type} `{Stringifiable A} `{EqClass A} (m : manifest_set A) :
+  list_InJson_to_manifest_set (manifest_set_to_list_InJson m) = resultC m.
+Proof.
+  induction m; simpl in *; intuition; eauto;
+  find_rewrite; rewrite canonical_stringification in *; simpl in *; eauto.
+Qed.
+
+Fixpoint manifest_set_pairs_to_list_InJson {A B : Type} `{Stringifiable A} 
+    `{Stringifiable B} (m : manifest_set (A * B)) : list InnerJSON :=
   match m with
   | [] => []
   | h :: t => 
         (pair_to_JSON_Array h) :: (manifest_set_pairs_to_list_InJson t)
   end.
 
-Fixpoint list_InJson_to_manifest_set_pairs {A B :Type} `{Serializable A} 
-    `{Serializable B} `{EqClass A} `{EqClass B}
+Fixpoint list_InJson_to_manifest_set_pairs {A B :Type} `{Stringifiable A} 
+    `{Stringifiable B} `{EqClass A} `{EqClass B}
     (l : list InnerJSON) : ResultT (manifest_set (A * B)) string :=
   match l with
   | nil => resultC []
@@ -346,9 +354,17 @@ Fixpoint list_InJson_to_manifest_set_pairs {A B :Type} `{Serializable A}
     match (InnerJSON_to_pair h) with
     | resultC h' =>
       match (list_InJson_to_manifest_set_pairs t) with
-      | resultC t' => resultC (manset_add h' t')
+      (* TODO: Same here as above, we would like to use add but it doesnt have all we need *)
+      | resultC t' => resultC (h' :: t')
       | errC e => errC e
       end
     | errC e => errC e
     end
   end.
+
+Lemma canonical_list_injson_to_manset_pairs {A B : Type} `{Stringifiable A, Stringifiable B} `{EqClass A, EqClass B} (m : manifest_set (A * B)) :
+  list_InJson_to_manifest_set_pairs (manifest_set_pairs_to_list_InJson m) = resultC m.
+Proof.
+  induction m; simpl in *; intuition; eauto;
+  find_rewrite; repeat rewrite canonical_stringification in *; simpl in *; eauto.
+Qed.
